\documentclass{article}

\usepackage{mathtools,amsfonts}
\usepackage{enumitem}
\usepackage{fullpage}
\usepackage{fancyvrb}
\usepackage{hyperref}
\usepackage{parskip}


\begin{document}
\thispagestyle{empty}

\begin{center}
  \textbf{\Large Advanced Solutions 4}
  % LEVEL is Senior, Intermediate or Beginner
  % NUMBER is the test number: 1, 2, etc.
  \\ \vspace{1em}
  \textbf{\large Stellenbosch Camp 2022}
  \\ \vspace{1em}
\end{center}

\bigskip \bigskip

\begin{enumerate}[itemsep=\fill]

\item % Source of problem
Problem statement


\item %
Show that $2022 \times 2^n$ can be written as the sum of three distinct non-zero squares for every natural number $n$.

\textbf{Solution:}
Note that $1011 = 31^2 + 7^2 + 1^2$ and $2022 = 43^2 + 13^2 + 2^2$.

If $n$ is odd, let $n = 2k + 1$. Then we have that
\[
    2022 \times 2^n = 1011 \times 2^{2k + 2} = \left( 31^2 + 7^2 + 1^2 \right) \times {\left( 2^{k + 1} \right)}^2 = {\left( 31 \times 2^{k + 1} \right)}^2 + {\left( 7 \times 2^{k + 1} \right)}^2 + {\left( 1 \times 2^{k + 1} \right)}^2.
\]

Similarly, if $n$ is even, let $n = 2k$. Then we have that
\[
    2022 \times 2^n = 2022 \times 2^{2k} = \left( 43^2 + 13^2 + 2^2 \right) \times {\left( 2^{k} \right)}^2 = {\left( 43 \times 2^{k} \right)}^2 + {\left( 13 \times 2^{k} \right)}^2 + {\left( 2 \times 2^{k} \right)}^2.
\]


\item % Andrew McGregor, 2022.
A triple of positive real numbers $(a,b,c)$ is called \textit{good} if $a,b,c$ are the side lengths of a non-degenerate triangle, and \textit{cute} if $a,b,c$ are the sides of an acute angled triangle. Prove that $(a,b,c)$ is \textit{good} if and only if $(\sqrt{a},\sqrt{b},\sqrt{c})$ is \textit{cute}. 

\textbf{Solution:}
Notice that if $(\sqrt{a},\sqrt{b},\sqrt{c})$ is \textit{cute}, then $\sqrt{a}^2 + \sqrt{b}^2 > \sqrt{c}^2$ for all permutatios of $(a,b,c)$ (Pythagoras' inequality) so $(\sqrt{a}^2,\sqrt{b}^2,\sqrt{c}^2)=(a,b,c)$ is \textit{good}.

If $(a,b,c)$ is good we note that it is sufficient to prove that $(\sqrt{a},\sqrt{b},\sqrt{c})$ is \textit{good} as Pythagoras' inequality would be trivialy satisfied. Use the Ravi substitution $a=x+y,b=y+z,c=z+x$ where $x,y,z>0$. Then
\begin{flalign*}
  \sqrt{a}+\sqrt{b} &= \sqrt{x+y} +\sqrt{y+z}\\
  &= \sqrt{\left( \sqrt{x+y} +\sqrt{y+z} \right)^2 }\\
  &= \sqrt{\left( x+y +y+z + 2\sqrt{(x+y)(y+z)}\right) }\\
  &= \sqrt{\left( x+z + (2y+ 2\sqrt{(x+y)(y+z)})\fight) }\\
  &> \sqrt{x+z}\\
  &= \sqrt{c}\\
\end{flalign*}
Similarly for $\sqrt{a}+\sqrt{c} >\sqrt{b}$ and $\sqrt{b}+\sqrt{c} >\sqrt{a}$.



\item % 


\item % 

\end{enumerate}

\end{document}
