\documentclass{article}

\usepackage{mathtools,amsfonts}
\usepackage{enumitem}
\usepackage{fullpage}
\usepackage{fancyvrb}
\usepackage{hyperref}
%\usepackage{parskip}


\begin{document}
\thispagestyle{empty}

\begin{center} \bfseries
  \Large Intermediate Test 5 Solutions
  \\ \vspace{12pt}
  \large Stellenbosch Camp 2022
\end{center}

\bigskip \bigskip

\begin{enumerate}[itemsep=24pt]

\item


\item


\item 



\item 


\item
Find all functions $f : \mathbb{R} \to \mathbb{R}$ such that \[ f(x+y) = f(x^2+y^2) \] for all $x,y \in \mathbb{R}$.

\textbf{Solution}:We see that making the substitution $y$ $\rightarrow$ $-x$ yields 
\begin{align}
    f(0)=f(2x^{2})
\end{align}
Consider any $a \in \mathbb{R}$, substitute $x$ $\rightarrow$ $\sqrt{\frac{a}{2}}$ into (1), this gives $f(0) = f(a)$ $\forall a \in \mathbb{R^{+}}$
\\Substituting $x$ $\rightarrow$ $-x$ and $y$ $\rightarrow$ $0$ into the original equation gives $f(-x) = f((-x)^{2}) = f(x^{2})$
\\Finally, substitute $y \rightarrow 0$ gives $f(x) = f(x^{2})$. Thus $f(x)= f(x^{2}) = f(-x)$ $\forall x \in \mathbb{R}$
\\Therefore $f(x) = f(0) = c$ $\forall x \in \mathbb{R}$ and the check is trivial.

\end{enumerate}

\end{document}
